CCS2/src/ObsCongrScript.sml
@@ -571,6 +571,22 @@ val OBS_CONGR_SUBST_RELAB = store_thm (
  >> IMP_RES_TAC WEAK_EQUIV_SUBST_RELAB
  >> ASM_REWRITE_TAC []);
 
+val OBS_CONGR_congruence = store_thm (
+   "OBS_CONGR_congruence",
+  ``!E E' ctx. CONTEXT ctx ==> OBS_CONGR E E' ==> OBS_CONGR (ctx E) (ctx E')``,
+    NTAC 2 GEN_TAC
+ >> HO_MATCH_MP_TAC CONTEXT_ind
+ >> BETA_TAC
+ >> REPEAT STRIP_TAC (* 7 sub-goals here *)
+ >> RES_TAC	     (* 6 sub-goals left *)
+ >| [ MATCH_MP_TAC OBS_CONGR_SUBST_PREFIX >> ASM_REWRITE_TAC [],
+      MATCH_MP_TAC OBS_CONGR_SUBST_SUM_R  >> ASM_REWRITE_TAC [],
+      MATCH_MP_TAC OBS_CONGR_SUBST_SUM_L  >> ASM_REWRITE_TAC [],
+      MATCH_MP_TAC OBS_CONGR_SUBST_PAR_R  >> ASM_REWRITE_TAC [],
+      MATCH_MP_TAC OBS_CONGR_SUBST_PAR_L  >> ASM_REWRITE_TAC [],
+      MATCH_MP_TAC OBS_CONGR_SUBST_RESTR  >> ASM_REWRITE_TAC [],
+      MATCH_MP_TAC OBS_CONGR_SUBST_RELAB  >> ASM_REWRITE_TAC [] ]);
+
 (******************************************************************************)
 (*                                                                            *)
 (*     Relationship between strong equivalence and observation congruence     *)
