CCS2/src/WeakEQScript.sml
@@ -7,6 +7,7 @@ open HolKernel Parse boolLib bossLib;
 
 open pred_setTheory relationTheory listTheory IndDefRules;
 open CCSLib CCSTheory StrongEQTheory;
+open cardinalTheory;
 
 val _ = new_theory "WeakEQ";
 
@@ -609,14 +610,7 @@ val WEAK_EQUIV = store_thm ((* NEW *)
       HO_MATCH_MP_TAC WEAK_EQUIV_coind \\ (* co-induction used here! *)
       PROVE_TAC [WEAK_BISIM] ]);
 
-val _ = set_mapped_fixity { fixity = Infix (NONASSOC, 450),
-			    tok = "=~", term_name = "WEAK_EQUIV" };
-
-val _ = Unicode.unicode_version { u = UTF8.chr 0x2248, tmnm = "WEAK_EQUIV"};
-val _ = TeX_notation { hol = UTF8.chr 0x2248,
-		       TeX = ("\\ensuremath{\\approx}", 1) };
-
-val _ = overload_on ("=~", ``WEAK_EQUIV``);
+val _ = overload_on ("=~", ``WEAK_EQUIV``); (* from cardinalTheory *)
 
 (******************************************************************************)
 (*									      *)
